feat: progress on macros
This includes a big update to the manual's syntax description DSL,
because it couldn't express quasiquotes before.

Manual/NotationsMacros.lean
@@ -7,10 +7,11 @@ Author: David Thrane Christiansen
 import VersoManual
 
 import Manual.Meta
-import Manual.Language.Classes
-import Manual.Language.Functions
-import Manual.Language.Files
-import Manual.Language.InductiveTypes
+import Manual.Papers
+
+import Manual.NotationsMacros.Operators
+import Manual.NotationsMacros.Precedence
+import Manual.NotationsMacros.Notations
 
 import Lean.Parser.Command
 
@@ -43,464 +44,12 @@ They can be combined flexibly to achieve the necessary results:
  * {ref "notations"}[Notations] allow the simultaneous definition of a parser extension, a macro, and a pretty printer.{TODO}[check the details on pretty printers and syntax vs notation]
  * Low-level parser extensions allow the parser to be extended in ways that modify its rules for tokens and whitespace, or that even completely replace Lean's syntax. This is an advanced topic that requires familiarity with Lean internals; nevertheless, the possibility of doing this without modifying the compiler is important. This reference manual is written using a language extension that replaces Lean's concrete syntax with a Markdown-like language for writing documents, but the source files are still Lean files.
 
-# Custom Operators
-%%%
-tag := "operators"
-%%%
+{include 0 Manual.NotationsMacros.Operators}
 
-Lean supports custom infix, prefix, and suffix operators.
-New operators can be added by any Lean library, and the new operators have equal status to those that are part of the language.
-Each new operator is assigned an interpretation as a function, after which uses of the operator are translated into uses of the function.
-The operator's translation into a function call is referred to as its {deftech}_expansion_.
-If this function is a {tech}[type class] {tech}[method], then the resulting operator can be overloaded by defining instances of the class.
+{include 0 Manual.NotationsMacros.Precedence}
 
-All operators have a {deftech}[precedence].
-Operator precedence determines the order of operations for unparenthesized expressions: because multiplication has a higher precedence than addition, {lean}`2 + 3 * 4` is equivalent to {lean}`2 + (3 * 4)`, and {lean}`2 * 3 + 4` is equivalent to {lean}`(2 * 3) + 4`.
-Infix operators additionally have an {deftech}[associativity] that determines the meaning of a chain of operators that have the same precedence:
+{include 0 Manual.NotationsMacros.Notations}
 
-: {deftech}[Left-associative]
-
-  These operators nest to the left.
-  Addition is left- associative, so {lean}`2 + 3 + 4 + 5` is equivalent to {lean}`((2 + 3) + 4) + 5`.
-
-: {deftech}[Right-associative]
-
-  These operators nest to the right.
-  The product type is right-associative, so {lean}`Nat × String × Unit × Option Int` is equivalent to {lean}`Nat × (String × (Unit × Option Int))`.
-
-: {deftech}[Non-associative]
-
-  Chaining these operators is a syntax error.
-  Explicit parenthesization is required.
-  Equality is non-associative, so the following is an error:
-
-  ```syntaxError eqs (category := term)
-  1 + 2 = 3 = 2 + 1
-  ```
-  The parser error is:
-  ```leanOutput eqs
-  <example>:1:10: expected end of input
-  ```
-::::keepEnv
-:::example "Precedence for Prefix and Infix Operators"
-```lean (show := false)
-axiom A : Prop
-axiom B : Prop
-example : (¬A ∧ B = (¬A) ∧ B) = (¬A ∧ ((B = ¬A) ∧ B)) := rfl
-example : (¬A ∧ B) = ((¬A) ∧ B) := rfl
-```
-
-The proposition {lean}`¬A ∧ B` is equivalent to {lean}`(¬A) ∧ B`, because `¬` has a higher precedence than `∧`.
-Because `∧` has higher precedence than `=` and is right-associative, {lean}`¬A ∧ B = (¬A) ∧ B` is equivalent to {lean}`¬A ∧ ((B = ¬A) ∧ B)`.
-:::
-::::
-
-Lean provides commands for defining new operators:
-:::syntax command
-Non-associative infix operators are defined using {keywordOf Lean.Parser.Command.mixfix}`infix`:
-```grammar
-$[$_:docComment]?
-$[$_:attributes]?
-$_:attrKind infix:$_ $[(name := $x)]? $[(priority := $_:prio)]? $s:str => $t:term
-```
-
-Left-associative infix operators are defined using {keywordOf Lean.Parser.Command.mixfix}`infixl`:
-```grammar
-$[$_:docComment]?
-$[$_:attributes]?
-$_:attrKind infixl:$_ $[(name := $x)]? $[(priority := $_:prio)]? $s:str => $t:term
-```
-
-Right-associative infix operators are defined using {keywordOf Lean.Parser.Command.mixfix}`infixr`:
-```grammar
-$[$_:docComment]?
-$[$_:attributes]?
-$_:attrKind infixr:$_ $[(name := $x)]? $[(priority := $_:prio)]? $s:str => $t:term
-```
-
-Prefix operators are defined using {keywordOf Lean.Parser.Command.mixfix}`prefix`:
-```grammar
-$[$_:docComment]?
-$[$_:attributes]?
-$_:attrKind prefix:$_ $[(name := $x)]? $[(priority := $_:prio)]? $s:str => $t:term
-```
-
-Postfix operators are defined using {keywordOf Lean.Parser.Command.mixfix}`postfix`:
-```grammar
-$[$_:docComment]?
-$[$_:attributes]?
-$_:attrKind postfix:$_ $[(name := $x)]? $[(priority := $_:prio)]? $s:str => $t:term
-```
-:::
-
-Each of these commands may be preceded by {tech}[documentation comments] and {tech}[attributes].
-The documentation comment is shown when the user hovers their mouse over the operator, and attributes may invoke arbitrary metaprograms, just as for any other declaration.
-The attribute {attr}`inherit_doc` causes the documentation of the function that implements the operator to be re-used for the operator itself.
-
-Operators interact with {tech}[section scopes] in the same manner as attributes.
-By default, operators are available in any module that transitively imports the one in which they are established, but they may be declared `scoped` or `local` to restrict their availability either to contexts in which the current namespace has been opened or to the current {tech}[section scope], respectively.
-
-Operators require a {ref "precedence"}[precedence] specifier, following a colon.
-There is no default precedence to fall back to for custom operators.
-
-Operators may be explicitly named.
-This name denotes the extension to Lean's syntax, and is primarily used for metaprogramming.
-If no name is explicitly provided, then Lean generates one based on the operator.
-The specifics of the assignment of this name should not be relied upon, both because the internal name assignment algorithm may change and because the introduction of similar operators in upstream dependencies may lead to a clash, in which case Lean will modify the assigned name until it is unique.
-
-::::keepEnv
-:::example "Assigned Operator Names"
-Given this infix operator:
-```lean
-@[inherit_doc]
-infix:90 " ⤴ " => Option.getD
-```
-the internal name {name}`«term_⤴_»` is assigned to the resulting parser extension.
-:::
-::::
-
-::::keepEnv
-:::example "Provided Operator Names"
-Given this infix operator:
-```lean
-@[inherit_doc]
-infix:90 (name := getDOp) " ⤴ " => Option.getD
-```
-the resulting parser extension is named {name}`getDOp`.
-:::
-::::
-
-:::TODO
-Describe the priority
-:::
-
-The actual operator is provided as a string literal.
-The new operator must satisfy the following requirements:
- * It must contain at least one character.
- * The first character may not be a single or double quote (`'` or `"`).
- * It may not begin with a backtick (``​`​``) followed by a character that would be a valid prefix of a quoted name.
- * It may not begin with a digit.
-
-The operator string literal may begin or end with a space.
-These are not part of the operator's syntax, and their presence does not require spaces around uses of the operator.
-However, the presence of spaces cause Lean to insert spaces when showing the operator to the user.
-Omitting them causes the operator's arguments to be displayed immediately next to the operator itself.
-
-
-:::keepEnv
-```lean (show := false)
--- Test claim about internal whitespace in preceding paragraph
-infix:99 " <<<< >>>> " => Nat.add
-
-/-- info: 67 -/
-#guard_msgs in
-#eval 12 <<<< >>>> 55
-
--- Test claim about internal whitespace
-infix:99 " <<<<  >>>> " => Nat.mul
-
-/-- info: 660 -/
-#guard_msgs in
-#eval 12 <<<<  >>>> 55
-
---- Test negative claims about allowed atoms
-/--
-error: invalid atom
----
-error: invalid syntax node kind 'bogus'
--/
-#guard_msgs in
-infix:9 (name := bogus) "" => Nat.mul
-
-#guard_msgs in
-infix:9 (name := nonbogus) " ` " => Nat.mul
-
-/--
-error: invalid atom
----
-error: invalid syntax node kind 'bogus'
--/
-#guard_msgs in
-infix:9 (name := bogus) "`a" => Nat.mul
-
-```
-:::
-
-Finally, the operator's meaning is provided, separated from the operator by {keywordOf Lean.Parser.Command.mixfix}`=>`.
-This may be any Lean term.
-Uses of the operator are desugared into function applications, with the provided term in the function position.
-Prefix and postfix operators apply the term to their single argument as an explicit argument.
-Infix operators apply the term to the left and right arguments, in that order.
-Other than its ability to accept arguments at each call site, there are no specific requirements imposed on the term.
-Operators may construct functions, so the term may expect more parameters than the operator.
-Implicit and {tech}[instance-implicit] parameters are resolved at each application site, which allows the operator to be defined by a {tech}[type class] {tech}[method].
-
-```lean (show := false) (keep := false)
--- Double-check claims about operators above
-prefix:max "blah" => Nat.add
-#check (blah 5)
-```
-
-If the term consists either of a name from the global environment or of an application of such a name to one or more arguments, then Lean automatically generates an {tech}[unexpander] for the operator.
-This means that the operator will be displayed in {tech}[proof states], error messages, and other output from Lean when the function term otherwise would have been displayed.
-Lean does not track whether the operator was used in the original term; it is inserted at every opportunity.
-
-:::::keepEnv
-::::example "Custom Operators in Lean's Output"
-The function {lean}`perhapsFactorial` computes a factorial for a number if it's not too large.
-```lean
-def fact : Nat → Nat
-  | 0 => 1
-  | n+1 => (n + 1) * fact n
-
-def perhapsFactorial (n : Nat) : Option Nat :=
-  if n < 8 then some (fact n) else none
-```
-
-The postfix interrobang operator can be used to represent it.
-```lean
-postfix:90 "‽" => perhapsFactorial
-```
-
-When attempting to prove that {lean}`∀ n, n ≥ 8 → (perhapsFactorial n).isNone`, the initial proof state uses the new operator, even though the theorem as written does not:
-```proofState
-∀ n, n ≥ 8 → (perhapsFactorial n).isNone := by skip
-/--
-⊢ ∀ (n : Nat), n ≥ 8 → n‽.isNone = true
--/
-
-```
-::::
-:::::
-
-# Precedences
-%%%
-tag := "precedence"
-%%%
-
-Infix operators, notations, and other syntactic extensions to Lean make use of explicit {tech}[precedence] annotations.
-While precedences in Lean can technically be any natural number, by convention they range from {evalPrec}`min` to {evalPrec}`max`, respectively denoted `min` and `max`.{TODO}[Fix the keywordOf operator and use it here]
-Function application has the highest precedence.
-
-:::syntax prec (open := false)
-Most operator precedences consist of explicit numbers.
-The named precedence levels denote the outer edges of the range, close to the minimum or maximum, and are typically used by more involved syntax extensions.
-```grammar
-$n:num
-```
-
-Precedences may also be denoted as sums or differences of precedences; these are typically used to assign precedences that are relative to one of the named precedences.
-```grammar
-$p + $p
-```
-```grammar
-$p - $p
-```
-```grammar
-($p)
-```
-
-The maximum precedence is used to parse terms that occur in a function position.
-Operators should typically not use use this level, because it can interfere with users' expectation that function application binds more tightly than any other operator, but it is useful in more involved syntax extensions to indicate how other constructs interact with function application.
-```grammar
-max
-```
-
-Argument precedence is one less than the maximum precedence.
-This level is useful for defining syntax that should be treated as an argument to a function, such as {keywordOf Lean.Parser.Term.fun}`fun` or {keywordOf Lean.Parser.Term.do}`do`.
-```grammar
-arg
-```
-
-Lead precedence is less that argument precedence, and should be used for custom syntax that should not occur as a function argument, such as {keywordOf Lean.Parser.Term.let}`let`.
-```grammar
-lead
-```
-
-The minimum precedence can be used to ensure that an operator binds less tightly than all other operators.
-```grammar
-min
-```
-:::
-
-# Notations
-%%%
-tag := "notations"
-%%%
-
-The term {deftech}_notation_ is used in two ways in Lean: it can refer to the general concept of concise ways of writing down ideas, and it is the name of a language feature that allows notations to be conveniently implemented with little code.
-Like custom operators, Lean notations allow the grammar of terms to be extended with new forms.
-However, notations are more general: the new syntax may freely intermix required keywords or operators with subterms, and they provide more precise control over precedence levels.
-Notations may also rearrange their parameters in the resulting subterms, while infix operators provide them to the function term in a fixed order.
-Because notations may define operators that use a mix of prefix, infix, and postfix components, they can be called {deftech}_mixfix_ operators.
-
-:::syntax command
-Notations are defined using the {keywordOf Lean.Parser.Command.notation}`notation` command.
-
-```grammar
-$[$_:docComment]?
-$[$_:attributes]?
-$_:attrKind notation$[:$_:prec]? $[(name := $_:ident)]? $[(priority := $_:prio)]? $[$_:notationItem]* => $_:term
-```
-:::
-
-:::syntax Lean.Parser.Command.notationItem (open := false)
-The body of a notation definition consists of a sequence of {deftech}_notation items_, which may be either string literals or identifiers with optional precedences.
-```grammar
-$s:str
-```
-```grammar
-$x:ident$[:$_:prec]?
-```
-:::
-
-As with operator declarations, the contents of the documentation comments are shown to users while they interact with the new syntax.
-Adding the {attr}`inherit_doc` attribute causes the documentation comment of the function at the head of the term into which the notation expands to be copied to the new syntax.
-Other attributes may be added to invoke other compile-time metaprograms on the resulting definition.
-
-Notations interact with {tech}[section scopes] in the same manner as attributes and operators.
-By default, notations are available in any module that transitively imports the one in which they are established, but they may be declared `scoped` or `local` to restrict their availability either to contexts in which the current namespace has been opened or to the current {tech}[section scope], respectively.
-
-:::TODO
-What is the priority?
-:::
-
-Rather than a single operator with its fixity and token, the body of a notation declaration consists of a sequence of {deftech}_notation items_, which may be either new {tech}[atoms] (including both keywords such as `if`, `#eval`, or `where` and symbols such as `=>`, `+`, `↗`, `⟦`, or `⋉`) or positions for terms.
-Just as they do in operators, string literals identify the placement of atoms.
-Leading and trailing spaces in the strings do not affect parsing, but they cause Lean to insert spaces in the corresponding position when displaying the syntax in {tech}[proof states] and error messages.
-Identifiers indicate positions where terms are expected, and name the corresponding term so it can be inserted in the notation's expansion.
-
-While custom operators have a single notion of precedence, there are many involved in a notation.
-The notation itself has a precedence, as does each term to be parsed.
-The notation's precedence determines which contexts it may be parsed in: the parser only attempts to parse productions whose precedence is at least as high as the current context.
-For example, because multiplication has higher precedence than addition, the parser will attempt to parse an infix multiplication term while parsing the arguments to addition, but not vice versa.
-The precedence of each term to be parsed determines which other productions may occur in them.
-
-If no precedence is supplied for the notation itself, the default value depends on the form of the notation.
-If the notation both begins and ends with an atom (represented by string literals), then the default precedence is `max`.{TODO}[keywordOf]
-This applies both to notations that consist only of a single atom and to notations with multiple items, in which the first and last items are both atoms.
-Otherwise, the default precedence of the whole notation is `lead`.
-If no precedence is provided for notation items that are terms, then they default to precedence `min`.
-
-```lean (keep := false) (show := false)
-
--- Test for default precedences for notations
-
-/-- Parser max -/
-notation "takesMax " e:max => e
-/-- Parser lead -/
-notation "takesLead " e:lead => e
-/-- Parser min -/
-notation "takesMin " e:min => e
-
-/-- Take the first one -/
-notation e1 " <# " e2 => e1
-
-/-- Take the first one in brackets! -/
-notation "<<<<<" e1 " <<# " e2 ">>>>>" => e1
-
-elab "#parse_test " "[" e:term "]"  : command => do
-  Lean.logInfoAt e (toString e)
-  pure ()
-
--- Here, takesMax vs takesLead distinguishes the notations
-
-/-- info: («term_<#_» (termTakesMax_ "takesMax" (num "1")) "<#" (num "2")) -/
-#guard_msgs in
-#parse_test [ takesMax 1 <# 2 ]
-
-/-- info: (termTakesLead_ "takesLead" («term_<#_» (num "1") "<#" (num "2"))) -/
-#guard_msgs in
-#parse_test [ takesLead 1 <# 2 ]
-
-
--- Here, takesMax vs takesLead does not distinguish the notations because both have precedence `max`
-
-/--
-info: (termTakesMax_ "takesMax" («term<<<<<_<<#_>>>>>» "<<<<<" (num "1") "<<#" (num "2") ">>>>>"))
--/
-#guard_msgs in
-#parse_test [ takesMax <<<<< 1 <<# 2 >>>>> ]
-
-/--
-info: (termTakesLead_ "takesLead" («term<<<<<_<<#_>>>>>» "<<<<<" (num "1") "<<#" (num "2") ">>>>>"))
--/
-#guard_msgs in
-#parse_test [ takesLead <<<<< 1 <<# 2 >>>>> ]
-```
-
-After the required double arrow ({keywordOf Lean.Parser.Command.notation}`=>`), the notation is provided with an expansion.
-While operators are always expanded by applying their function to the operator's arguments in order, notations may place their term items in any position in the expansion.
-The terms are referred to by name.
-Term items may occur any number of times in the expansion.
-Because notation expansion is a purely syntactic process that occurs prior to elaboration or code generation, duplicating terms in the expansion may lead to duplicated computation when the resulting term is evaluated, or even duplicated side effects when working in a monad.
-
-::::keepEnv
-:::example "Ignored Terms in Notation Expansion"
-This notation ignores its first parameter:
-```lean
-notation (name := ignore) "ignore " _ign:arg e:arg => e
-```
-
-The term in the ignored position is discarded, and Lean never attempts to elaborate it, so terms that would otherwise result in errors can be used here:
-```lean (name := ignore)
-#eval ignore (2 + "whatever") 5
-```
-```leanOutput ignore
-5
-```
-
-However, the ignored term must still be syntactically valid:
-```syntaxError ignore' (category := command)
-#eval ignore (2 +) 5
-```
-```leanOutput ignore'
-<example>:1:17: expected term
-```
-:::
-::::
-
-::::keepEnv
-:::example "Duplicated Terms in Notation Expansion"
-
-The {keywordOf dup}`dup!` notation duplicates its sub-term.
-
-```lean
-notation (name := dup) "dup!" t:arg => (t, t)
-```
-
-Because the term is duplicated, it can be elaborated separately with different types:
-```lean
-def e : Nat × Int := dup! (2 + 2)
-```
-
-Printing the resulting definition demonstrates that the work of addition will be performed twice:
-```lean (name := dup)
-#print e
-```
-```leanOutput dup
-def e : Nat × Int :=
-(2 + 2, 2 + 2)
-```
-:::
-::::
-
-
-When the expansion consists of the application of a function defined in the global environment and each term in the notation occurs exactly once, an {tech}[unexpander] is generated.
-The new notation will be displayed in {tech}[proof states], error messages, and other output from Lean when matching function application terms otherwise would have been displayed.
-As with custom operators, Lean does not track whether the notation was used in the original term; it is used at every opportunity in Lean's output.
-
-## Operators and Notations
-%%%
-tag := "operators-and-notations"
-%%%
-
-Internally, operator declarations are translated into notation declarations.
-Term notation items are inserted where the operator would expect arguments, and in the corresponding positions in the expansion.
-For prefix and postfix operators, the notation's precedence as well as the precedences of its term items is the operator's declared precedence.
-For non-associative infix operators, the notation's precedence is the declared precedence, but both arguments are parsed at a precedence level that is one higher, which prevents successive uses of the notation without parentheses.
-Associative infix operators use the operator's precedence for the notation and for one argument, while a precedence that is one level higher is used for the other argument; this prevents successive applications in one direction only.
-Left-associative operators use the higher precedence for their right argument, while right-associative operators use the higher precedence for their left argument.
 
 # Defining New Syntax
 
@@ -762,9 +311,10 @@ Attributes may be added to invoke compile-time metaprograms on the resulting def
 Syntax rules interact with {tech}[section scopes] in the same manner as attributes, operators, and notations.
 By default, syntax rules are available to the parser in any module that transitively imports the one in which they are established, but they may be declared `scoped` or `local` to restrict their availability either to contexts in which the current namespace has been opened or to the current {tech}[section scope], respectively.
 
-:::TODO
-What is the priority?
-:::
+When multiple syntax rules for a category can match the current input, the {tech}[local longest-match rule] is used to select one of them.
+Like notations and operators, if there is a tie for the longest match then the declared priorities are used to determine which parse result applies.
+If this still does not resolve the ambiguity, then all the results that tied are saved.
+The elaborator is expected to attempt all of them, succeeding when exactly one can be elaborated.
 
 The syntax rule's precedence, written immediately after the {keywordOf Lean.Parser.Command.syntax}`syntax` keyword, restricts the parser to use this new syntax only when the precedence context is at least the provided value.
 {TODO}[Default precedence]
@@ -920,8 +470,6 @@ tag := "macros"
 %%%
 
 :::planned 71
- * Definition of {deftech}_macro_
- * {deftech}_Macro expansion_
  * `macro_rules`
    * Syntax patterns
    * Backtracking on expansion failure
@@ -929,6 +477,515 @@ tag := "macros"
  * The `macro` command
 :::
 
+{deftech}_Macros_ are transformations from {name Lean.Syntax}`Syntax` to {name Lean.Syntax}`Syntax` that occur during {tech key:="elaborator"}[elaboration] and during {ref "tactic-macros"}[tactic execution].
+Replacing syntax with the result of transforming it with a macro is called {deftech}_macro expansion_.
+Multiple macros may be associated with a single {tech}[syntax kind], and they are attempted in order of definition.
+Macros are run in a {tech}[monad] that has access to some compile-time metadata and has the ability to either emit an error message or to delegate to subsequent macros, but the macro monad is much less powerful than the elaboration monads.
+
+```lean (show := false)
+section
+open Lean (Syntax MacroM)
+```
+
+Macros are associated with {tech}[syntax kinds].
+An internal table maps syntax kinds to macros of type {lean}`Syntax → MacroM Syntax`.
+Macros delegate to the next entry in the table by throwing the {name Lean.Macro.Exception.unsupportedSyntax}`unsupportedSyntax` exception.
+A given {name}`Syntax` value _is a macro_ when there is a macro associated with its syntax kind that does not throw {name Lean.Macro.Exception.unsupportedSyntax}`unsupportedSyntax`.
+If a macro throws any other exception, an error is reported to the user.
+{tech}[Syntax categories] are irrelevant to macro expansion; however, because each syntax kind is typically associated with a single syntax category, they do not interfere in practice.
+
+::::keepEnv
+:::example "Macro Error Reporting"
+The following macro reports an error when its parameter is the literal numeral five.
+It expands to its argument in all other cases.
+```lean
+syntax &"notFive" term:arg : term
+open Lean in
+macro_rules
+  | `(term|notFive 5) => Macro.throwError "'5' is not allowed here"
+  | `(term|notFive $e) => pure e
+```
+
+When applied to terms that are not syntactically the numeral five, elaboration succeeds:
+```lean (name := notFiveAdd)
+#eval notFive (2 + 3)
+```
+```leanOutput notFiveAdd
+5
+```
+
+When the error case is triggered, the user receives an error message:
+```lean (name := notFiveFive) (error := true)
+#eval notFive 5
+```
+```leanOutput notFiveFive
+'5' is not allowed here
+```
+:::
+::::
+
+Before elaborating a piece of syntax, the elaborator checks whether its {tech}[syntax kind] has macros associated with it.
+These are attempted in order.
+If a macro succeeds, potentially returning syntax with a different kind, the check is repeated and macros are expanded again until the outermost layer of syntax is no longer a macro.
+Elaboration or tactic execution can then proceed.
+Only the outermost layer of syntax (typically a {name Lean.Syntax.node}`node`) is expanded, and the output of macro expansion may contain nested syntax that is a macro.
+These nested macros are expanded in turn when the elaborator reaches them.
+
+```lean (keep := false) (show := false)
+-- Test claim in preceding paragraph that it's OK for macros to give up prior to elab
+syntax "doubled " term:arg : term
+
+macro_rules
+  | `(term|doubled $n:num) => `($n * 2)
+  | `(term|doubled $_) => Lean.Macro.throwUnsupported
+
+/-- info: 10 -/
+#guard_msgs in
+#eval doubled 5
+
+/--
+error: elaboration function for 'termDoubled_' has not been implemented
+  doubled (5 + 2)
+-/
+#guard_msgs in
+#eval doubled (5 + 2)
+
+elab_rules : term
+  | `(term|doubled $e:term) => Lean.Elab.Term.elabTerm e none
+
+/-- info: 7 -/
+#guard_msgs in
+#eval doubled (5 + 2)
+```
+
+## Hygiene
+%%%
+tag := "macro-hygiene"
+%%%
+
+A macro is {deftech (key:="hygiene")}_hygienic_ if its expansion cannot result in identifier capture.
+{deftech}[Identifier capture] is when an identifier ends up referring to a binding site other than that which is in scope where the identifier occurs in the source code.
+There are two types of identifier capture:
+ * If a macro's expansion introduces binders, then identifiers that are parameters to the macro may end up referring to the introduced binders if their names happen to match.
+ * If a macro's expansion is intended to refer to a name, but the macro is used in a context that either locally binds this name or in which a new global name has been introduced, it may end up referring to the wrong name.
+
+The first kind of variable capture can be avoided by ensuring that every binding introduced by a macro uses a freshly generated, globally-unique name, while the second can be avoided by always using fully-qualified names to refer to constants.
+The fresh names must be generated again at each invocation of the macro to avoid variable capture in recursive macros.
+These techniques are error-prone.
+Variable capture issues are difficult to test for because they rely on coincidences of name choices, and consistently applying these techniques results in noisy code.
+
+Lean features automatic hygiene: in almost all cases, macros are automatically hygienic.
+Capture by introduced bindings is avoided by annotating identifiers introduced by a macro with {deftech}_macro scopes_, which uniquely identify each invocation of macro expansion.
+If the binding and the use of the identifier have the same macro scopes, then they were introduced by the same step of macro expansion and should refer to one another.
+Similarly, uses of global names in code generated by a macro are not captured by local bindings in the context in which they are expanded because these use sites have macro scopes that are not present in the binding occurrence.
+Capture by newly-introduced global names are prevented by annotating potential global name references with the set of matching globals in code produced in the macro's body.
+Identifiers annotated with potential referents are called {deftech}_pre-resolved identifiers_, and the {lean}`Syntax.Preresolved` field on the {name}`Syntax.ident` constructor is used to store the potential referents.
+
+The introduction of macro scopes and pre-resolved identifiers to generated syntax occurs during {tech}[quotation].
+Macros that construct syntax by other means than quotation should also ensure hygiene by some other means.
+For more details on Lean's hygiene algorithm, please consult {citet beyondNotations ullrich23}[].
+
+## The Macro Monad
+%%%
+tag := "macro-monad"
+%%%
+
+The macro monad {name Lean.MacroM}`MacroM` is sufficiently powerful to implement hygiene and report errors.
+Macro expansion does not have the ability to modify the environment directly, to carry out unification, to examine the current local context, or to do anything else that only makes sense in one particular context.
+This allows the same macro mechanism to be used throughout Lean, and it makes macros much easier to write than {tech}[elaborators].
+
+{docstring Lean.MacroM}
+
+{docstring Lean.Macro.expandMacro?}
+
+{docstring Lean.Macro.trace}
+
+### Exceptions and Errors
+%%%
+tag := "macro-exceptions"
+%%%
+
+The {name Lean.Macro.Exception.unsupportedSyntax}`unsupportedSyntax` exception is used for control flow during macro expansion.
+It indicates that the current macro is incapable of expanding the received syntax, but that an error has not occurred.
+The exceptions thrown by {name Lean.Macro.throwError}`throwError` and {name Lean.Macro.throwErrorAt}`throwErrorAt` terminate macro expansion, reporting the error to the user.
+
+{docstring Lean.Macro.throwUnsupported}
+
+{docstring Lean.Macro.Exception.unsupportedSyntax}
+
+{docstring Lean.Macro.throwError}
+
+{docstring Lean.Macro.throwErrorAt}
+
+### Hygiene-Related Operations
+%%%
+tag := "macro-monad-hygiene"
+%%%
+
+{tech}[Hygiene] is implemented by adding {tech}[macro scopes] to the identifiers that occur in syntax.
+Ordinarily, the process of {tech}[quotation] adds all necessary scopes, but macros that construct syntax directly must add macro scopes to the identifiers that they introduce.
+
+{docstring Lean.Macro.withFreshMacroScope}
+
+{docstring Lean.Macro.addMacroScope}
+
+### Querying the Environment
+%%%
+tag := "macro-environment"
+%%%
+
+Macros have only limited support for querying the environment.
+They can check whether a constant exists and resolve names, but further introspection is unavailable.
+
+{docstring Lean.Macro.hasDecl}
+
+{docstring Lean.Macro.getCurrNamespace}
+
+{docstring Lean.Macro.resolveNamespace}
+
+{docstring Lean.Macro.resolveGlobalName}
+
+## Quasiquotation
+%%%
+tag := "quasiquotation"
+%%%
+
+{deftech}_Quotation_ marks code for representation as data of type {name}`Syntax`.
+Quoted code is parsed, but not elaborated—while it must be syntactically correct, it need not make sense.
+Quotation makes it much easier to programmatically generate code: rather than reverse-engineering the specific nesting of {name Lean.Syntax.node}`node` values that Lean's parser would produce, the parser can be directly invoked to create them.
+This is also more robust in the face of refactoring of the grammar that may change the internals of the parse tree without affecting the user-visible concrete syntax.
+Quotation in Lean is surrounded by ``​`(`` and `)`.
+
+The syntactic category or parser being quoted may be indicated by placing its name after the opening backtick and parenthesis, followed by a vertical bar (`|`).
+As a special case, the name `tactic` may be used to parse either tactics or sequences of tactics.
+If no syntactic category or parser is provided, Lean attempts to parse the quotation both as a term and as a non-empty sequence of commands.
+Term quotations have higher priority than command quotations, so in cases of ambiguity, the interpretation as a term is chosen; this can be overridden by explicitly indicating that the quotation is of a command sequence.
+
+::::keepEnv
+:::example "Term vs Command Quotation Syntax"
+```lean (show := false)
+open Lean
+```
+
+In the following example, the contents of the quotation could either be a function application or a sequence of commands.
+Both match the same region of the file, so the {tech}[local longest-match rule] is not relevant.
+Term quotation has a higher priority than command quotation, so the quotation is interpreted as a term.
+Terms expect their {tech}[antiquotations] to have type {lean}``TSyntax `term`` rather than {lean}``TSyntax `command``.
+```lean (error := true) (name := cmdQuot)
+example (cmd1 cmd2 : TSyntax `command) : MacroM (TSyntax `command) := `($cmd1 $cmd2)
+```
+The result is two type errors like the following:
+```leanOutput cmdQuot
+application type mismatch
+  cmd1.raw
+argument
+  cmd1
+has type
+  TSyntax `command : Type
+but is expected to have type
+  TSyntax `term : Type
+```
+
+The type of the quotation ({lean}``MacroM (TSyntax `command)``) is not used to select a result because syntax priorities are applied prior to elaboration.
+In this case, specifying that the antiquotations are commands resolves the ambiguity because function application would require terms in these positions:
+```lean
+example (cmd1 cmd2 : TSyntax `command) : MacroM (TSyntax `command) := `($cmd1:command $cmd2:command)
+```
+Similarly, inserting a command into the quotation eliminates the possibility that it could be a term:
+```lean
+example (cmd1 cmd2 : TSyntax `command) : MacroM (TSyntax `command) := `($cmd1 $cmd2 #eval "hello!")
+```
+:::
+::::
+
+```lean (show := false)
+-- There is no way to extract parser priorities (they're only saved in the Pratt tables next to
+-- compiled Parser code), so this test of priorities checks the observable relative priorities of the
+-- quote parsers.
+
+/--
+info: do
+  let _ ← Lean.MonadRef.mkInfoFromRefPos
+  let _ ← Lean.getCurrMacroScope
+  let _ ← Lean.getMainModule
+  pure { raw := { raw := Syntax.missing }.raw } : MacroM (Lean.TSyntax `term)
+-/
+#guard_msgs in
+#check (`($(⟨.missing⟩)) : MacroM _)
+/--
+info: do
+  let info ← Lean.MonadRef.mkInfoFromRefPos
+  let _ ← Lean.getCurrMacroScope
+  let _ ← Lean.getMainModule
+  pure
+      {
+        raw :=
+          Syntax.node2 info `Lean.Parser.Term.app { raw := Syntax.missing }.raw
+            (Syntax.node1 info `null { raw := Syntax.missing }.raw) } : MacroM (Lean.TSyntax `term)
+-/
+#guard_msgs in
+#check (`($(⟨.missing⟩) $(⟨.missing⟩)) : MacroM _)
+/--
+info: do
+  let info ← Lean.MonadRef.mkInfoFromRefPos
+  let _ ← Lean.getCurrMacroScope
+  let _ ← Lean.getMainModule
+  pure
+      {
+        raw :=
+          Syntax.node2 info `null { raw := Syntax.missing }.raw
+            { raw := Syntax.missing }.raw } : MacroM (Lean.TSyntax `command)
+-/
+#guard_msgs in
+#check (`($(⟨.missing⟩):command $(⟨.missing⟩)) : MacroM _)
+
+/--
+info: do
+  let _ ← Lean.MonadRef.mkInfoFromRefPos
+  let _ ← Lean.getCurrMacroScope
+  let _ ← Lean.getMainModule
+  pure { raw := { raw := Syntax.missing }.raw } : MacroM (Lean.TSyntax `tactic)
+-/
+#guard_msgs in
+#check (`(tactic| $(⟨.missing⟩):tactic) : MacroM _)
+
+/--
+info: do
+  let info ← Lean.MonadRef.mkInfoFromRefPos
+  let _ ← Lean.getCurrMacroScope
+  let _ ← Lean.getMainModule
+  pure
+      {
+        raw :=
+          Syntax.node1 info `Lean.Parser.Tactic.seq1
+            (Syntax.node3 info `null { raw := Syntax.missing }.raw (Syntax.atom info ";")
+              { raw := Syntax.missing }.raw) } : MacroM (Lean.TSyntax `tactic.seq)
+-/
+#guard_msgs in
+#check (`(tactic|
+          $(⟨.missing⟩):tactic; $(⟨.missing⟩)) : MacroM _)
+```
+
+:::freeSyntax term (open := false)
+
+Lean's syntax includes quotations for terms, commands, tactics, and sequences of tactics, as well as a general quotation syntax that allows any input that Lean can parse to be quoted.
+Term quotations have the highest priority, followed by tactic quotations, general quotations, and finally command quotations.
+
+```grammar
+`(term|`($_:term))
+*******
+"`("$_:command+")"
+*******
+`(term|`(tactic| $_:tactic))
+*******
+`(term|`(tactic| $_:tactic;*))
+*******
+"`("p:ident"|"/-- Parse a {p} here -/")"
+```
+:::
+
+```lean (show := false)
+section M
+variable {m : Type → Type}
+open Lean (MonadRef MonadQuotation)
+open Lean.Elab.Term (TermElabM)
+open Lean.Elab.Command (CommandElabM)
+open Lean.Elab.Tactic (TacticM)
+```
+
+Rather than having type {name}`Syntax`, quotations are monadic actions with type {lean}`m Syntax`.
+Quotation is monadic because it implements {tech}[hygiene] by adding {tech}[macro scopes] and preresolving identifiers, as described in {ref "macro-hygiene"}[the section on hygiene].
+The specific monad to be used is an implicit parameter to the quotation, and any monad for which there is an instance of the {name}`MonadQuotation` type classe is suitable.
+{name}`MonadQuotation` extends {name}`MonadRef`, which gives the quotation access to the source location of the syntax that the macro expander or elaborator is currently processing. {name}`MonadQuotation` additionally includes the ability to add {tech}[macro scopes] to identifiers and use a fresh macro scope for a sub-task.
+Monads that support quotation include {name}`MacroM`, {name}`TermElabM`, {name}`CommandElabM`, and {name}`TacticM`.
+
+```lean (show := false)
+end M
+```
+
+
+```lean (show := false)
+-- Verify claim about monads above
+open Lean in
+example [Monad m] [MonadQuotation m] : m Syntax := `(term|2 + 2)
+```
+
+{deftech}_Quasiquotation_ is a form of quotation that may contain {deftech}_antiquotations_, which are regions of the quotation that are not quoted, but instead are expressions that are evaluated to yield syntax.
+A quasiquotation is essentially a template; the outer quoted region provides a fixed framework that always yields the same outer syntax, while the antiquotations yield the parts of the final syntax that vary.
+All quotations in Lean are quasiquotations, so no special syntax is needed to distinguish quasiquotations from other quotations.
+
+Basic antiquotations consist of a dollar sign (`$`) followed by an identifier.
+This means that the identifier's value, which should be a syntax tree, is to be substituted into this position of the quoted syntax.
+Entire expressions may be used as antiquotations by wrapping them in parentheses.
+
+```lean (show := false)
+section
+open Lean
+example (e : Term) : MacroM Syntax := `(term| $e)
+
+example (e : Term) : MacroM Syntax := `(term| $(e))
+
+--example (e : Term) : MacroM Syntax := `(term| $ (e))
+
+
+end
+```
+
+
+
+```lean (show := false)
+section
+open Lean (TSyntax SyntaxNodeKinds)
+variable {c : SyntaxNodeKinds}
+```
+
+Lean's parser assigns every antiquotation a syntax category based on what the parser expects at the given position.
+If the parser expects syntax category {lean}`c`, then the antiquotation's type must be {lean}`TSyntax c`.
+Some syntax categories can be matched by elements of other categories.
+For example, numeric and string literals are valid terms in addition to being their own syntax categories.
+Antiquotations may be annotated with the expected category, which causes the parser to validate that the annotated category is acceptable in the given position and construct any intermediate layers that are required in the parse tree.
+
+::::keepEnv
+:::example "Antiquotation Annotations"
+```lean (show := false)
+open Lean
+```
+
+This example requires that {lean}`m` is a monad that can perform quotation.
+```lean
+variable {m : Type → Type} [Monad m] [MonadQuotation m]
+```
+
+By default, the antiquotation `$e` is expected to be a term, because that's the syntactic category that's immediately expected as the second argument to addition.
+```lean (name := ex1)
+def ex1 (e) := show m _ from `(2 + $e)
+#check ex1
+```
+```leanOutput ex1
+ex1 {m : Type → Type} [Monad m] [MonadQuotation m] (e : TSyntax `term) : m (TSyntax `term)
+```
+
+Annotating `$e` as a numeric literal succeeds, because numeric literals are also valid terms.
+The expected type of the parameter `e` changes to ``TSyntax `num``.
+```lean (name := ex2)
+def ex2 (e) := show m _ from `(2 + $e:num)
+#check ex2
+```
+```leanOutput ex2
+ex2 {m : Type → Type} [Monad m] [MonadQuotation m] (e : TSyntax `num) : m (TSyntax `term)
+```
+:::
+::::
+
+```lean (show := false)
+end
+```
+
+Antiquotations also support optionality and repetition with optional separators.
+
+
+::::keepEnv
+:::example "Repetition Annotations"
+```lean (show := false)
+open Lean
+```
+
+This example requires that {lean}`m` is a monad that can perform quotation.
+```lean
+variable {m : Type → Type} [Monad m] [MonadQuotation m]
+```
+
+By default, the antiquotation `$e` is expected to be an array of terms separated by commas, as is expected in the body of a list:
+```lean (name := ex1)
+def ex1 (xs) := show m _ from `(#[$xs,*])
+#check ex1
+```
+```leanOutput ex1
+ex1 {m : Type → Type} [Monad m] [MonadQuotation m] (xs : Syntax.TSepArray `term ",") : m (TSyntax `term)
+```
+
+However, Lean includes a collection of coercions between various representations of arrays that will automatically insert or remove separators, so an ordinary array of terms is also acceptable:
+```lean (name := ex2)
+def ex2 (xs : Array (TSyntax `term)) := show m _ from `(#[$xs,*])
+#check ex2
+```
+```leanOutput ex2
+ex2 {m : Type → Type} [Monad m] [MonadQuotation m] (xs : Array (TSyntax `term)) : m (TSyntax `term)
+```
+
+:::
+::::
+
+```lean (show := false)
+section
+open Lean Syntax
+variable {k k' : SyntaxNodeKinds} {sep : String} [Coe (TSyntax k) (TSyntax k')]
+-- Demonstrate the coercions between different kinds of repeated syntax
+
+/-- info: instCoeHTCTOfCoeHTC -/
+#guard_msgs in
+#synth CoeHTCT (TSyntaxArray k) (TSepArray k sep)
+
+/-- info: instCoeHTCTOfCoeHTC -/
+#guard_msgs in
+#synth CoeHTCT (TSyntaxArray k) (TSepArray k' sep)
+
+/-- info: instCoeHTCTOfCoeHTC -/
+#guard_msgs in
+#synth CoeHTCT (Array (TSyntax k)) (TSepArray k sep)
+
+/-- info: instCoeHTCTOfCoeHTC -/
+#guard_msgs in
+#synth CoeHTCT (TSepArray k sep) (TSyntaxArray k)
+
+end
+```
+
+:::freeSyntax antiquot (open := true) (title := "Token Antiquotations")
+
+Token antiquotations replace the source information (of type {name Lean.SourceInfo}`SourceInfo`) on a token with the source information from some other syntax.
+
+```grammar
+str"%$"ident
+```
+:::
+
+::: TODO
+Syntax of antiquotes (requires hack)
+
+All kinds of antiquotes:
+ * `$x`
+ * `$x:cat`
+ * `$(tm)`
+ * `$x\*`
+ * `$[$x]?/*,`
+ * `"foo"%$tk`
+:::
+
+
+:::example "Quasiquotation"
+
+Both forms of antiquotation are used in this example.
+Because natural numbers are not syntax, {name Lean.quote}`quote` is used to transform a number into syntax that represents it.
+
+```lean
+open Lean in
+example [Monad m] [MonadQuotation m] (x : Term) (n : Nat) : m Syntax :=
+  `($x + $(quote (n + 2)))
+```
+:::
+
+::::keepEnv
+:::example "Expanding Quasiquotation"
+```lean
+open Lean in
+def f [Monad m] [MonadQuotation m] (x : Term) (n : Nat) : m Syntax :=
+  `(fun k => $x + $(quote (n + 2)) + k)
+#print f
+```
+
+:::
+::::
 
 ## Matching Syntax
 
